paper/other-prims.scrbl
@@ -1,0 +1,186 @@
+#lang scribble/base
+@(require "util.rkt" "cite.rkt"
+          "../rkt/sub1-plot.rkt"
+          (prefix-in p: plot/pict)
+          scriblib/figure
+	  scriblib/footnote
+          "../rkt/diff-sub-div-plot.rkt")
+
+@title{Other Uses of Arithmetic}
+
+Our case study contains other uses of arithmetic operations that
+treat operations on BigNums as constant when they are not. This
+section discusses them. None of the proofs in this section
+have been formalized in Coq.
+
+@section{The @raw-latex{$\log$}-time @tt{size} function}
+ 
+The @raw-latex{$\log$}-time @tt{size} function for Braun trees,
+reproduced below, performs an addition in each recursive
+call that is not tracked within the monad. Performing the
+sum, @raw-latex{$1 + (2*m) + zo$}, cannot always be
+replaced by a constant time operation. The Braun tree
+invariant, however, guarantees that @raw-latex{$zo$} is
+either 0 or 1 because it is the difference in size between
+the left and right subtrees of a Braun tree. Therefore, in
+the worst case, evaluating @raw-latex{$1 + (2*m) + zo$}
+requires time proportional to @raw-latex{$\log{m}$}.
+Evaluating @tt{diff s m} to compute @raw-latex{$zo$} also
+requires time proportional to @raw-latex{$\log{m}$}.
+Therefore, ignoring the time complexity of the addition
+operation does not affect our analysis of the @tt{size}
+function's running time.
+
+@(apply inline-code (extract size_log_sq_gen.v cdr))
+
+@section{Subtraction and Division Together}
+
+The copy functions, such as @tt{copy_log_sq}, exhibit a more complicated recursion pattern.
+These functions apply two primitives
+for each recursive call, subtraction by 1 and division by 2. It is not obvious that
+this combination of operations is safe to ignore in run time calculations because whereas
+@tt{div2} is a constant time operation, subtracting by 1, as we have already seen, is not.
+
+@(apply inline-code (extract copy_log_sq_gen.v cdr))
+
+We argue by strong induction that for any binary number, if we perform a sequence of
+@tt{sub1} and @tt{div2} operations, the running time of the combination
+is amortized constant time. More strongly, we claim that the total
+runtime of performing @tt{sub1} and @tt{div2} operations on a binary number
+@raw-latex{$b$} until we reach 0 is @raw-latex{$3n$}, where we count iterations of
+@tt{sub1} and @tt{div2} as a single unit of time and @raw-latex{$n$} is the number of
+bits in @raw-latex{$b$}.
+
+For the proof, consider a binary number @raw-latex{$b$}. If
+@raw-latex{$b$} is zero the result is trivial. If
+@raw-latex{$b$} is odd then there exists some @raw-latex{$b'
+ < b$} such that @raw-latex{$b = 2*b'+1$}. As a list of bits,
+@raw-latex{$b$} is represented by a 1 followed by the bits
+in @raw-latex{$b'$}. We write this representation as
+@raw-latex{$b = 1 \cdot b'$} to make the lower order bits,
+upon which subtraction and division operate, explicit.
+Performing a sequence of @tt{sub1} and @tt{div2} operations
+on @raw-latex{$b = 1 \cdot b'$} takes 2 units of time (1
+each for @tt{sub1} and @tt{div2}) to reduce to @raw-latex{
+ $b'$} plus the time to perform the sequence of operations on
+@raw-latex{$b'$}. By induction, we have that performing @tt{
+ sub1} and @tt{div2} operations on @raw-latex{$b'$} will take
+at most @raw-latex{$3*(n-1)$} units of time. Adding these
+together, the sequence of operations takes no more than
+@raw-latex{$3n$} units of time in total.
+
+In the even case, for a non-zero binary number @raw-latex{
+ $b$} of @raw-latex{$n$} bits, the list representation of
+@raw-latex{$b$} must begin with some number, @raw-latex{
+ $k$}, of zeros followed by a 1 and then the representation
+of some smaller binary number. Therefore, there exists a
+@raw-latex{$b'$} such that @raw-latex{$b = 0 \cdots 0 \cdot
+ 1 \cdot b'$} with @raw-latex{$k \leq n$} zeros at the front
+of the number. Subtracting 1 from this number takes
+@raw-latex{$k+1$} units of time, therefore one combination
+of subtraction and division takes @raw-latex{$k+2$} units of
+time and results in a number of the form @raw-latex{$1
+ \cdots 1 \cdot 0 \cdot b'$} with @raw-latex{$k-1$} ones at
+the front of the list. It is clear that the next @raw-latex{
+ $k-1$} iterations will each take 2 units of time. Thus, to
+reduce to the number @raw-latex{$0 \cdot b'$} of length
+@raw-latex{$n-k$} takes @raw-latex{$3k$} units of time.
+Finally, applying the induction hypothesis to the smaller
+number @raw-latex{$0 \cdot b'$} completes the proof.
+	
+This proof shows that repeatedly subtracting by 1 and
+dividing by 2 in each recursive call and terminating at 0
+requires time that is linear in the number of recursive
+calls. Therefore, each use of subtraction followed by
+division takes amortized constant time in functions such as
+@tt{copy_log_sq}, and ignoring these primitive operations
+does not affect our analysis of their running time.
+
+This proof has not been formalized in Coq.
+
+@figure["fig:diff-sub-div"
+	@list{Average running time of @tt{sub1} and @tt{div2}}
+	@diff-sub/div-plot]
+
+@section{Branching with Subtraction and Division}
+
+The fourth problematic recursion pattern appears in the implementation
+of @tt{diff}, reproduced below. In the body of the last pattern
+match, (@tt{bt_node x s t, S m'}), the function branches on the parity
+of its input, @raw-latex{$m$}, and if the input is even subtracts 2
+then divides by 2, in the odd case we see the recursion described
+above of subtracting 1 then dividing by 2. Clearly, if control flow
+never reaches the even case then these operations are constant time
+and we may safely ignore them. If the evaluation of @tt{diff} does
+reach the even case, however, then we must be certain that the
+subtraction and division operations do not change our
+analysis. Subtracting 1 twice from an even number takes logarithmic
+time in the worst case. The first subtraction may traverse the entire
+number, but the second subtraction is from an odd number and takes
+constant time. @Figure-ref["fig:diff-sub-div"] presents a plot of the
+average@note{The average here is the total amount of abstract time used
+by the primitive operations in a call to @tt{diff} divided by the
+number of recursive calls.} amount of abstract time required by
+subtraction and division in each recursive call of @tt{diff}. Although
+the graph only extends from 0 to 1024 this pattern extends to larger
+numbers as well. The plot suggests that primitive operations used by
+@tt{diff} could be characterized. We speculate it requires only
+amortized constant time, although it appears less than linear. The
+plot suggests that a proof of this claim should be possible, but we
+leave the detailed analysis and formalization to future work.
+
+@(apply inline-code (extract diff_gen.v cdr))
+
+
+@figure["fig:copy_linear-input"
+        @list{Running time of @tt{copy_linear}}
+        (parameterize ([p:plot-width 275]
+                       [p:plot-height 275]
+                       [p:plot-x-label "Copy_linear's Input"]
+                       [p:plot-y-label "Sub1 Calls' Running Time"])
+          ;; this plot takes a long time, but I like that last steep jump...
+          (plot-with-bound 10000
+                           copy_linear_sub1_points
+                           copy_linear_sub1_bound))]
+
+@section{A Tree of Subtraction and Division}
+
+Finally, the most complicated pattern is that used by @tt{copy_linear},
+which recursively calls itself on @tt{n/2} and
+@tt{(n-1)/2}. @Figure-ref["fig:copy_linear-input"] is a plot of the
+running time of the @tt{sub1} calls that @tt{copy_linear} makes. In
+gray is a plot of @raw-latex{$\lambda x. 31x + 29$}, which we believe
+is an upper bound for the function. Proving that the uses of @tt{div2}
+and @tt{sub1} in this function contribute only a linear factor to the
+overall runtime is a significant challenge. Compared to our proof that
+the primitive operations in functions like @tt{copy_log_sq} which deals with
+a linear sequence of operations, a proof for the primitive operations in
+@tt{copy_linear} must consider a tree of all possible sequences of the operations
+that evaluate @tt{n/2} and @tt{(n-1)/2}. A similar proof should be possible with
+the insight that each expensive computation of @tt{(n-1)/2} takes the same number
+of operations to reach the next expensive computation regardless of the path taken
+down the tree, however, we have not attempted a formal proof of this claim.
+
+@(apply inline-code (extract copy_linear_gen.v cdr))
+
+@section{Primitive Operations Cost Recap}
+
+The informal analysis presented above suggests that, although we have
+not accounted for all language primitives, our calculations of
+asymptotic run times remain unchanged. We have presented arguments
+that support that it is safe to ignore certain uses of language
+primitives, providing proof where possible and suggesting directions
+for more formal arguments in the remaining cases. A goal of our future
+work is to formalize these arguments in Coq.
+
+An alternative approach is to assign a symbolic constant to the the
+cost of each one of these primitives following @citet[jost-carbon] and
+@citet[aspinall-program]. This amounts to a vector-based cost
+semantics where each element of the vector records the number of times
+the corresponding operation is used. Since this is compositionally
+additive, it may be used in place of our default semantics. This
+approach would lend itself well to experimentally estimating the
+costs, to formalize them separated, or to collapsing them into
+units (as we do in the present version).
+
+
