paper/prims.scrbl
@@ -1,12 +1,10 @@
 #lang scribble/base
 @(require "util.rkt" "cite.rkt"
           "../rkt/sub1-plot.rkt"
-          (prefix-in : "../arith/sub1_gen.rkt")
           (prefix-in p: plot/pict)
           scriblib/figure
 	  scriblib/footnote
-          pict 
-          (prefix-in c: scribble/core)
+          pict
           "../rkt/diff-sub-div-plot.rkt")
 
 @title[#:tag "sec:prims"]{Accounting for Language Primitives}
@@ -19,7 +17,7 @@ functions (e.g., @tt{car} and @tt{cdr}) are certainly constant
 time. Structure allocation functions (e.g., @tt{cons}) are usually
 constant time when using a two-space copying collector, as most
 garbage-collected languages do. Occasionally, allocation triggers
-garbage collection, which we can assume amortized constant time (but not
+garbage collection, which we can assume is amortized constant time (but not
 something our framework handles).
 
 More interestingly, and more often overlooked, however, are
@@ -45,60 +43,79 @@ time. However, certain uses of addition can be replaced by
 constant-time bit operations. For instance, doubling and
 adding 1 can be replaced by a specialized operation that
 conses a @tt{1} on the front of the bitstring. The remainder
-of this section examines each of uses of arithmetic operations
-that occur in our case study.
+of this section explores how BigNum arithmetic affects
+the running time computations of various functions.
 
-@section{Using Addition and Subtraction to Recur}
+@section[#:tag "sec:add-and-subtract"]{Addition and Subtraction}
 
-A common pattern for functions that consume a natural number
-is to count up or count down, adding 1 or subtracting 1 at
-each recursive step. For example, in the extracted OCaml
-code for @tt{fib}, pattern matching against @tt{S} @tt{n}
-becomes a call to the @tt{pred_big_int} function.
-Subtracting 1 from a number represented in binary requires
-more than constant time; @tt{sub1} may need to traverse the
-entire number to compute its predecessor in the general
-case.
+To get us started, here is the implementation of @tt{sub1} in
+terms of constant-time BigNum operations, written in our monad:
 
-To be certain that the non-constant run time of @tt{sub1} does not affect our
-calculation of the run time, we argue that the implicit subtractions
-hiding inside pattern matching take amortized constant time.
+@(apply inline-code (extract sub1_gen.v cdr))
+
+where @tt{sub1_result} asserts that the result of
+the function is one less than the input and
+that the running time is a function in @raw-latex{$O(\log(n))$}.
+
+The use of @tt{n - 1} may seem strange in the last line
+of the function, but in that case we know that @tt{n} is
+odd, so that operation corresponds to zeroing the last
+bit of the number, a constant time operation.
+
+Unlike the conventional implementation of on Peano arithmetic,
+this function is not constant time. Specifically, if the
+@tt{if} expression always takes the true branch, then
+the function will traverse the entire representation of the
+number. This possible path through the function is why it
+takes @raw-latex{$\log$} time; the representation of the number
+takes space proportional to @raw-latex{$\log$} of its value.
+
+In addition to @tt{sub1},
+our library contains implementations of @tt{add1}, addition,
+and multiplication, together with proofs that
+@tt{add1} is  @raw-latex{$O(\log(n))$},
+addition is
+@raw-latex{$\Theta(\log(\max(m,n)))$}, and
+multiplication is
+@raw-latex{$\Theta(\log(n)\cdot(log(m)+\log(n)))$}.
+
+@section{Using Subtraction to Recur}
+
+A common pattern for functions in our case study is to consume a natural number
+and count down, subtracting 1 at
+each recursive step. A naive analysis based on the result in
+@secref["sec:add-and-subtract"] suggests that this could add
+a @raw-latex{$\log$} factor to the running time, but that is
+not a tight bound.
+
 Although subtraction by 1 is not always a constant time operation, it is
-constant time on half of its possible inputs. That is, on any odd number represented
-in binary, subtracting by 1 is a constant time operation. It follows
-that any number equivalent to 2 modulo 4 will require 2 units of time
+constant time on half of its possible inputs. That is, on any odd number,
+subtracting by 1 is a constant time operation. Similarly,
+any number equivalent to 2 modulo 4 will require 2 units of time
 to perform the @tt{sub1} operation because @tt{sub1} will terminate after two
-iterations. In general, there is a
-@(c:element (c:style "relax" '(exact-chars)) '("\\(\\frac{1}{2^n}\\)"))
-chance that @tt{sub1} terminates after 
-@(c:element (c:style "relax" '(exact-chars)) '("\\(n\\)"))
-iterations. To account for all uses of @tt{sub1} in the implementation of
-@tt{fib}, we note that we will perform the @tt{sub1} operation on each number
+iterations. In general, there is a @raw-latex{\(\frac{1}{2^n}\)}
+chance that @tt{sub1} terminates after @raw-latex{\(n\)} iterations.
+
+To account for all uses of @tt{sub1} in the implementation of a
+function that counts down, we note that we perform the @tt{sub1} operation on each number
 from 1 to @raw-latex{$n$}. This gives a cost in terms of the iterations required by
 @tt{sub1} that is bounded above by
 @raw-latex{$n*(\frac{1}{2} + \frac{2}{4} + \frac{3}{8} + \cdots + \frac{n}{2^n} + \cdots$)}.
 One can show that this infinite sum converges to @raw-latex{$2*n$}, thus for a sequence of
-@raw-latex{$n$} @tt{sub1} operations this shows
-that subtraction implicit in the definition of @tt{fib} requires amortized constant time.
-Overall, the run time of the additions performed by @tt{fib}
-will dwarf the time required by subtraction. This justifies the fact that we do not
-explicitly consider the time taken by @tt{sub1} operations.
+@raw-latex{$n$} @tt{sub1} operations require amortized constant time.
 
-The @tt{add1} operation is dual to @tt{sub1}; on every even
-number adding 1 is a constant time operation whereas
-subtracting 1 is constant time on odd numbers. Therefore the
-same argument we apply to show that @tt{sub1} takes
-amortized constant time applies to @tt{add1}. We have not
-formalized this proof in Coq.
+We have proved this using our monad, showing that this function is linear time:
+
+@(apply inline-code (extract sub1_linear_loop_gen.v cdr))
 
 @section{Addition in Fib}
 
-The uses of addition in @tt{fib} are not constant time. We
-did not account for the time of additions in the recursive
-implementation of @tt{fib}. We did prove (in Coq), however,
+We did not account for the time of additions in the
+recursive implementation of @tt{fib}. We did prove, however,
 that the iterative @tt{fib} function, which requires linear
-time when additions are not counted, requires quadratic time
-when we properly account for primitive operations.
+time when additions are considered constant time, requires
+quadratic time when we properly account for primitive
+operations.
 
 Addition has a run time that is linear in the
 number of bits of its input. Using this fact, we can prove that
@@ -117,17 +134,20 @@ quadratic lower bound.  Since the other primitives used in calculating
 addition operations, and thus the run time of @tt{fib} is bounded
 below by a factor of @raw-latex{$n^2$}.
 
-A similar argument shows that the run time of @tt{fib} has a quadratic upper bound.
-Combining these two results proves that the run time of the iterative version of @tt{fib}
-is asymptotically @raw-latex{$n^2$} when we account for primitive operations.
+A similar argument shows that the run time of @tt{fib} has a
+quadratic upper bound. Combining these two results proves
+that the run time of the iterative version of @tt{fib} is
+@raw-latex{$\Theta(n^2)$} when we properly account for
+primitive operations.
 
-The supplementary material contains proofs of these facts in Coq (@tt{fib/fib_iter.v}).
+The supplementary material contains proofs of these facts in
+Coq (@tt{fib/fib_iter.v}).
 
-@section{Operations on Braun Trees}
 
-Functions that operate on Braun trees, such as @tt{size_linear} (reproduced below) and
-@tt{size_log_sq} have addition patterns like
-@raw-latex{$lsize + rsize + 1$} that are not obviously constant time operations.
+@section{The @tt{size_linear} Function}
+
+The @tt{size_linear} function, reproduced below has the addition expression
+@raw-latex{$lsize + rsize + 1$} that is not obviously a constant time operation.
 The Braun tree invariant, however, allows for an efficient implementation
 of this addition. The invariant requires either that @raw-latex{$lsize = rsize$}
 or @raw-latex{$lsize = rsize + 1$}. In the former case, the addition corresponds
@@ -139,174 +159,20 @@ of the list of bits. In either situation the addition
 operation can be transformed into a constant time operation and therefore does not
 invalidate our calculation of the running time of the @tt{size_linear} function.
 
-@(apply inline-code (extract size_linear_gen.v cdr))
+On the left is the Okasaki's original linear time @tt{size} function, translated
+into Coq and on the right is a version that uses only constant-time BigNum operations.
 
-Similarly, the @tt{size} function for Braun trees,
-reproduced below, performs an addition in each recursive
-call that is not tracked within the monad. Performing the
-sum, @raw-latex{$1 + (2*m) + zo$}, can not always be
-replaced by a constant time operation. The Braun tree
-invariant, however, guarantees that @raw-latex{$zo$} is
-either 0 or 1 because it is the difference in size between
-the left and right subtrees of a Braun tree. Therefore, in
-the worst case, evaluating @raw-latex{$1 + (2*m) + zo$}
-requires time proportional to @raw-latex{$\log{m}$}.
-Evaluating @tt{diff s m} to compute @raw-latex{$zo$} also
-requires time proportional to @raw-latex{$\log{m}$}.
-Therefore, ignoring the time complexity of the addition
-operation does not affect our analysis of the @tt{size}
-function's running time.
+@tabular[(let ([lines1 (extract size_linear_gen.v cdr)]
+               [lines2 (extract size_linear_bin_gen.v cdr)])
+           (list
+            (list
+             (apply inline-code
+                    "\n"
+                    (append
+                     lines1
+                     (build-list (- (length lines2) (length lines1)) (λ (i) "\n"))))
+             (apply inline-code "\n" lines2))))]
 
-@(apply inline-code (extract size_log_sq_gen.v cdr))
-
-@section{Subtraction and Division Together}
-
-The copy functions, such as @tt{copy_log_sq}, exhibit a more complicated recursion pattern.
-These functions apply two primitives
-for each recursive call, subtraction by 1 and division by 2. It is not obvious that
-this combination of operations is safe to ignore in run time calculations because whereas
-@tt{div2} is a constant time operation, subtracting by 1, as we have already seen, is not.
-
-@(apply inline-code (extract copy_log_sq_gen.v cdr))
-
-We argue by strong induction that for any binary number, if we perform a sequence of
-@tt{sub1} and @tt{div2} operations, the running time of the combination
-is amortized constant time. More strongly, we claim that the total
-runtime of performing @tt{sub1} and @tt{div2} operations on a binary number
-@raw-latex{$b$} until we reach 0 is @raw-latex{$3n$}, where we count iterations of
-@tt{sub1} and @tt{div2} as a single unit of time and @raw-latex{$n$} is the number of
-bits in @raw-latex{$b$}.
-
-For the proof, consider a binary number @raw-latex{$b$}. If
-@raw-latex{$b$} is zero the result is trivial. If
-@raw-latex{$b$} is odd then there exists some @raw-latex{$b'
- < b$} such that @raw-latex{$b = 2*b'+1$}. As a list of bits,
-@raw-latex{$b$} is represented by a 1 followed by the bits
-in @raw-latex{$b'$}. We write this representation as
-@raw-latex{$b = 1 \cdot b'$} to make the lower order bits,
-upon which subtraction and division operate, explicit.
-Performing a sequence of @tt{sub1} and @tt{div2} operations
-on @raw-latex{$b = 1 \cdot b'$} takes 2 units of time (1
-each for @tt{sub1} and @tt{div2}) to reduce to @raw-latex{
- $b'$} plus the time to perform the sequence of operations on
-@raw-latex{$b'$}. By induction, we have that performing @tt{
- sub1} and @tt{div2} operations on @raw-latex{$b'$} will take
-at most @raw-latex{$3*(n-1)$} units of time. Adding these
-together, the sequence of operations takes no more than
-@raw-latex{$3n$} units of time in total.
-
-In the even case, for a non-zero binary number @raw-latex{
- $b$} of @raw-latex{$n$} bits, the list representation of
-@raw-latex{$b$} must begin with some number, @raw-latex{
- $k$}, of zeros followed by a 1 and then the representation
-of some smaller binary number. Therefore, there exists a
-@raw-latex{$b'$} such that @raw-latex{$b = 0 \cdots 0 \cdot
- 1 \cdot b'$} with @raw-latex{$k \leq n$} zeros at the front
-of the number. Subtracting 1 from this number takes
-@raw-latex{$k+1$} units of time, therefore one combination
-of subtraction and division takes @raw-latex{$k+2$} units of
-time and results in a number of the form @raw-latex{$1
- \cdots 1 \cdot 0 \cdot b'$} with @raw-latex{$k-1$} ones at
-the front of the list. It is clear that the next @raw-latex{
- $k-1$} iterations will each take 2 units of time. Thus, to
-reduce to the number @raw-latex{$0 \cdot b'$} of length
-@raw-latex{$n-k$} takes @raw-latex{$3k$} units of time.
-Finally, applying the induction hypothesis to the smaller
-number @raw-latex{$0 \cdot b'$} completes the proof.
-	
-This proof shows that repeatedly subtracting by 1 and
-dividing by 2 in each recursive call and terminating at 0
-requires time that is linear in the number of recursive
-calls. Therefore, each use of subtraction followed by
-division takes amortized constant time in functions such as
-@tt{copy_log_sq}, and ignoring these primitive operations
-does not affect our analysis of their running time.
-
-This proof has not been formalized in Coq.
-
-@figure["fig:diff-sub-div"
-	@list{Average running time of @tt{sub1} and @tt{div2}}
-	@diff-sub/div-plot]
-
-@section{Branching with Subtraction and Division}
-
-The fourth problematic recursion pattern appears in the implementation
-of @tt{diff}, reproduced below. In the body of the last pattern
-match, (@tt{bt_node x s t, S m'}), the function branches on the parity
-of its input, @raw-latex{$m$}, and if the input is even subtracts 2
-then divides by 2, in the odd case we see the recursion described
-above of subtracting 1 then dividing by 2. Clearly, if control flow
-never reaches the even case then these operations are constant time
-and we may safely ignore them. If the evaluation of @tt{diff} does
-reach the even case, however, then we must be certain that the
-subtraction and division operations do not change our
-analysis. Subtracting 1 twice from an even number takes logarithmic
-time in the worst case. The first subtraction may traverse the entire
-number, but the second subtraction is from an odd number and takes
-constant time. @Figure-ref["fig:diff-sub-div"] presents a plot of the
-average@note{The average here is the total amount of abstract time used
-by the primitive operations in a call to @tt{diff} divided by the
-number of recursive calls.} amount of abstract time required by
-subtraction and division in each recursive call of @tt{diff}. Although
-the graph only extends from 0 to 1024 this pattern extends to larger
-numbers as well. The plot suggests that primitive operations used by
-@tt{diff} could be characterized. We speculate it requires only
-amortized constant time, although it appears less than linear. The
-plot suggests that a proof of this claim should be possible, but we
-leave the detailed analysis and formalization to future work.
-
-@(apply inline-code (extract diff_gen.v cdr))
-
-
-@figure["fig:copy_linear-input"
-        @list{Running time of @tt{copy_linear}}
-        (parameterize ([p:plot-width 275]
-                       [p:plot-height 275]
-                       [p:plot-x-label "Copy_linear's Input"]
-                       [p:plot-y-label "Sub1 Calls' Running Time"])
-          ;; this plot takes a long time, but I like that last steep jump...
-          (plot-with-bound 10000
-                           copy_linear_sub1_points
-                           copy_linear_sub1_bound))]
-
-@section{A Tree of Subtraction and Division}
-
-Finally, the most complicated pattern is that used by @tt{copy_linear},
-which recursively calls itself on @tt{n/2} and
-@tt{(n-1)/2}. @Figure-ref["fig:copy_linear-input"] is a plot of the
-running time of the @tt{sub1} calls that @tt{copy_linear} makes. In
-gray is a plot of @raw-latex{$\lambda x. 31x + 29$}, which we believe
-is an upper bound for the function. Proving that the uses of @tt{div2}
-and @tt{sub1} in this function contribute only a linear factor to the
-overall runtime is a significant challenge. Compared to our proof that
-the primitive operations in functions like @tt{copy_log_sq} which deals with
-a linear sequence of operations, a proof for the primitive operations in
-@tt{copy_linear} must consider a tree of all possible sequences of the operations
-that evaluate @tt{n/2} and @tt{(n-1)/2}. A similar proof should be possible with
-the insight that each expensive computation of @tt{(n-1)/2} takes the same number
-of operations to reach the next expensive computation regardless of the path taken
-down the tree, however, we have not attempted a formal proof of this claim.
-
-@(apply inline-code (extract copy_linear_gen.v cdr))
-
-@section{Primitive Operations Cost Recap}
-
-The informal analysis presented above suggests that, although we have
-not accounted for all language primitives, our calculations of
-asymptotic run times remain unchanged. We have presented arguments
-that support that it is safe to ignore certain uses of language
-primitives, providing proof where possible and suggesting directions
-for more formal arguments in the remaining cases. A goal of our future
-work is to formalize these arguments in Coq.
-
-An alternative approach is to assign a symbolic constant to the the
-cost of each one of these primitives following @citet[jost-carbon] and
-@citet[aspinall-program]. This amounts to a vector-based cost
-semantics where each element of the vector records the number of times
-the corresponding operation is used. Since this is compositionally
-additive, it may be used in place of our default semantics. This
-approach would lend itself well to experimentally estimating the
-costs, to formalize them separated, or to collapsing them into
-units (as we do in the present version).
-
-
+We proved both of them have the same running time (where the
+primitive operations in each count as unit time) and both
+compute the correct result.
